The user wants a clear explanation of the steps involved in combining the two first-order differential equations (`dV/dx = -rI` and `dI/dx = -gV`) to obtain the second-order differential equations for voltage (`V`) and current (`I`) independently.

**Plan:**
1.  Start with the two established first-order equations.
2.  Derive the second-order equation for `V`:
    *   Take the derivative of the first equation (`dV/dx = -rI`) with respect to `x`.
    *   Substitute the second equation (`dI/dx = -gV`) into the result.
    *   Simplify to get `d²V/dx² = (rg)V`.
3.  Derive the second-order equation for `I`:
    *   Take the derivative of the second equation (`dI/dx = -gV`) with respect to `x`.
    *   Substitute the first equation (`dV/dx = -rI`) into the result.
    *   Simplify to get `d²I/dx² = (rg)I`.
4.  Clearly state the resulting pair of second-order equations.