Okay, let's focus on achieving the specific goal: **Understanding *how* the differential equations derived for the leaky current path lead directly to solutions involving `cosh` and `sinh`.**

Here's the step-by-step connection:

1.  **Recall the Differential Equations:**
    We established that for a conductor with distributed resistance `r` (per unit length) and distributed leakage conductance `g` (per unit length) through passivation, the voltage `V(x)` and current `I(x)` at position `x` satisfy these second-order linear differential equations:
    *   `d²V/dx² = (r * g) * V(x)`
    *   `d²I/dx² = (r * g) * I(x)`

2.  **Simplify the Notation:**
    Let's define a constant `α² = r * g`. Since `r` and `g` are positive physical quantities, `α²` is positive. Let `α = sqrt(r * g)`. This `α` is real and positive, often called the attenuation constant.
    The differential equations become:
    *   `d²V/dx² = α² * V(x)`
    *   `d²I/dx² = α² * I(x)`
    Both voltage and current obey the same mathematical form: `d²y/dx² = α²y`.

3.  **Find the General Solution (Standard Method using Exponentials):**
    This is a standard type of differential equation. We look for solutions of the form `y = e^(kx)`.
    *   Substitute `y = e^(kx)` into `d²y/dx² = α²y`.
    *   The first derivative is `dy/dx = k * e^(kx)`.
    *   The second derivative is `d²y/dx² = k² * e^(kx)`.
    *   Substituting into the DE: `k² * e^(kx) = α² * e^(kx)`.
    *   Since `e^(kx)` is never zero, we can divide by it, leaving the **characteristic equation**: `k² = α²`.
    *   The roots of this equation are `k = +α` and `k = -α`.
    *   Because we have two distinct real roots, the general solution is a linear combination of the two corresponding exponential functions:
        `y(x) = C₁ * e^(αx) + C₂ * e^(-αx)`
        where `C₁` and `C₂` are arbitrary constants determined by the specific boundary conditions of the problem (e.g., voltage at the start, current at the end).
    *   So, specifically for voltage and current:
        `V(x) = C₁ * e^(αx) + C₂ * e^(-αx)`
        `I(x) = C₃ * e^(αx) + C₄ * e^(-αx)`
        *(Note: The constants `C₁`, `C₂`, `C₃`, `C₄` are not all independent; they are linked by the original first-order equations `dV/dx = -rI` and `dI/dx = -gV`)*

4.  **Transform the Solution to Hyperbolic Functions:**
    This is the key step connecting the exponential solution to `cosh` and `sinh`. We use the fundamental definitions of the hyperbolic functions:
    *   `cosh(u) = (e^u + e^-u) / 2`
    *   `sinh(u) = (e^u - e^-u) / 2`
    We can rearrange these to express the exponentials:
    *   Adding the two definitions: `cosh(u) + sinh(u) = e^u`
    *   Subtracting the second from the first: `cosh(u) - sinh(u) = e^-u`

    Now, substitute these expressions for `e^(αx)` and `e^(-αx)` back into our general solution `y(x) = C₁e^(αx) + C₂e^(-αx)`:
    `y(x) = C₁ * [cosh(αx) + sinh(αx)] + C₂ * [cosh(αx) - sinh(αx)]`

    Distribute the constants `C₁` and `C₂`:
    `y(x) = C₁*cosh(αx) + C₁*sinh(αx) + C₂*cosh(αx) - C₂*sinh(αx)`

    Group the terms containing `cosh(αx)` and `sinh(αx)`:
    `y(x) = (C₁ + C₂) * cosh(αx) + (C₁ - C₂) * sinh(αx)`

5.  **Introduce New Constants:**
    Since `C₁` and `C₂` are arbitrary constants, the combinations `(C₁ + C₂)` and `(C₁ - C₂)` are also just arbitrary constants. Let's rename them for clarity:
    *   Let `A = C₁ + C₂`
    *   Let `B = C₁ - C₂`
    The general solution can now be written equivalently as:
    `y(x) = A * cosh(αx) + B * sinh(αx)`

    Therefore, the general solutions for voltage and current can be expressed as:
    *   `V(x) = A * cosh(αx) + B * sinh(αx)`
    *   `I(x) = C * cosh(αx) + D * sinh(αx)`
    *(Again, the constants A, B, C, D are determined by boundary conditions and are related to each other through the physics of the system expressed in the first-order DEs).*

**Conclusion:**

The hyperbolic functions `cosh(αx)` and `sinh(αx)` arise not as fundamentally different solutions, but as a direct algebraic rearrangement of the standard exponential solution (`C₁e^(αx) + C₂e^(-αx)`) to the second-order differential equation `d²y/dx² = α²y`. This form using `cosh` and `sinh` is often more convenient for applying boundary conditions (especially at x=0) and interpreting the physical behaviour in terms of symmetric (cosh) and anti-symmetric (sinh) components, aligning well with transmission line theory.